\documentclass{article}

\usepackage{amsmath, amsthm, amsfonts, mathtools}
\usepackage{enumitem}
\usepackage[margin=1in]{geometry}

\begin{document}


\subsection*{1a}
\begin{align*}
X &\sim Exp(\frac{1}{10})\\
p(X<4.5) &= \int_{0}^{4.5} \frac{1}{10}e^{-\frac{x}{10}}dx\\
&= -e^{-0.1x} \Big|_0^{4.5}\\
&= -e^{-0.1 \cdot 4.5} + 1\\
&= 0.362
\end{align*}


\subsection*{1c}
\begin{align*}
0.8 &= \int_{0}^{a} \frac{1}{10}e^{-\frac{x}{10}}dx\\
0.8 &= -e^{-0.1x} \Big|_0^{a}\\
0.8 &= -e^{-0.1a} + 1\\
0.2 &= e^{-0.1a}\\
a &= \frac{\ln0.2}{-0.1}\\
a &= 16.0944
\end{align*}


\subsection*{1d}
\begin{align*}
	X &\sim Exp(\frac{1}{10})\\
	\mathbb{E}(X) &= \frac{1}{\lambda}\\
								&= \frac{1}{0.1} \\
								&= 10
\end{align*}


\subsection*{2a}
\begin{align*}
\int_{0}^{1} 12x^2(1-x)dx &= \int_{0}^{1} 12x^2-12x^3dx\\
													&= 4x^3 - 3x^4 \Big|_0^1\\
													&= 4 - 3\\
													&= 1
\end{align*}


\subsection*{2b}
\begin{align*}
	\int_{0}^{1} x\cdot12x^2(1-x)dx &= \int_{0}^{1} 12x^3-12x^4dx\\
																	&= 3x^4 - \frac{12}{5}x^5 \Big|_0^1\\
																	&= 3 - \frac{12}{5}\\
																	&= \frac{3}{5}
\end{align*}


\subsection*{3}
Since the probability density function of the uniform distribution is a constant
$\frac{1}{4-0} = 0.25$, propogating this distribution through the polynomial can
be done through convolution:
\begin{align*}
	\int_{0}^{4}0.25(3x^2 + 4x - 1)dx &= 0.25\left[x^3 + 2x^2 -x \right]^4_0\\
																		&= 0.25(4^3 + 2\cdot 4^2 - 3)\\
																		&= 23
\end{align*}


\subsection*{4}
\begin{align*}
	0.75 &= \int_0^a \lambda e ^{-\lambda x}\\
	0.75 &= -e ^{-\lambda x}\Big|_0^a\\
	0.75 &= -e^{-\lambda a} + 1\\
	0.25 &= e^{-\lambda a}\\
	a &= \frac{-\ln 0.25}{\lambda}
\end{align*}


\subsection*{5}
\begin{align*}
	Var(X) &= \mathbb{E}[X^2] - \mathbb{E}[X]^2\\
	&= \int_a^b \frac{1}{b-a}x^2 dx - (\frac{a+b}{2})^2\\
	&= \frac{1}{b-a} \int_a^bx^2 dx - (\frac{a+b}{2})^2\\
	&= \frac{1}{b-a}\left[\frac{x^3}{3}\right]_a^b - (\frac{a+b}{2})^2\\
	&= \frac{b^3 - a^3}{3(b-a)} - (\frac{a+b}{2})^2\\
	&= \frac{a^2 + ab + b^2}{3} - \frac{a^2 + 2ab + b^2}{4}\\
	&= \frac{a^2 - 2ab + b^2}{12}\\
	&= \frac{(b-a)^2}{12}
\end{align*}


\subsection*{6}
\begin{align*}
	p(X > 3) &= \lim_{n \to \infty} \int_3^n \frac{1}{5} e^{-0.2x} dx\\
	&= \lim_{n \to \infty} \left[-e^{-0.2x}\right]_3^n\\
	&= \lim_{n \to \infty}[-e^{-0.2n} + e^{-0.2 \cdot 3}]\\
	&= e^{-0.6}\\
	&= 0.549
\end{align*}

\end{document}

